theories/simulang/simple_inv/refl.v
@@ -62,4 +62,13 @@ Section refl.
     intros ?. iApply gen_log_rel_ctx; first by apply simple_log_rel_structural. done.
   Qed.
 
+  Lemma log_rel_func x e_t e_s :
+    free_vars e_t ∪ free_vars e_s ⊆ {[x]} →
+    log_rel e_t e_s -∗
+    func_rel (x, e_t) (x, e_s).
+  Proof.
+    apply gen_log_rel_func.
+    iIntros (v_t v_s π). rewrite /= left_id. eauto.
+  Qed.
+
 End refl.
